kami-rv32im: use primitive FIFOs in the processor impl.

Kami/PrimFifo.v
@@ -7,38 +7,6 @@ Set Implicit Arguments.
 
 Definition primFifoName: string := "FIFO".
 
-Section ListAsFifo.
-  Variable (sz: nat).
-  Context {dType: Kind}.
-
-  Definition listIsEmpty {ty} (l: list (ty dType)) :=
-    match l with
-    | nil => ConstBool true
-    | _ => ConstBool false
-    end.
-  
-  Definition listIsFull {ty} (l: list (ty dType)) :=
-    if eq_nat_dec (List.length l) sz
-    then ConstBool true
-    else ConstBool false.
-  
-  Definition listEnq {ty} (a: ty dType) (l: list (ty dType)) :=
-    l ++ [a].
-
-  Definition listDeq {ty} (l: list (ty dType)) :=
-    match l with
-    | nil => nil
-    | h :: t => t
-    end.
-  
-  Definition listFirstElt {ty} (l: list (ty dType)): Expr ty (SyntaxKind dType) :=
-    match l with
-    | nil => ($$Default)%kami_expr
-    | h :: t => (#h)%kami_expr
-    end.
-
-End ListAsFifo.
-
 Section PrimFifo.
   Variables (fifoName: string)
             (sz: nat)
@@ -46,97 +14,131 @@ Section PrimFifo.
 
   Local Notation "^ s" := (fifoName -- s) (at level 0).
 
-  Definition fifoEltT ty := list (ty dType).
-  Definition fifoEltK ty := @NativeKind (fifoEltT ty) nil.
-  Definition fifoElt ty := (^"elt" :: (@NativeConst (fifoEltT ty) nil nil))%struct.
-
-  Definition fifoEnq: forall ty (d: ty dType), ActionT ty Void :=
-    fun ty d =>
-      (ReadN eltT : fifoEltK ty <- ^"elt";
-       Assert !$$(listIsFull sz eltT);
-       Write ^"elt" <- (Var _ (fifoEltK ty) (listEnq d eltT));
+  Definition fifoEnq: MethodT {| arg := dType; ret := Void |} :=
+    fun _ d =>
+      (Read isFull <- ^"full";
+       Assert !#isFull;
+       Write ^"elt" <- #d;
+       Write ^"full" <- $$true;
        Retv)%kami_action.
 
-  Definition fifoDeq: forall ty (_: ty Void), ActionT ty dType :=
-    fun ty _ =>
-      (ReadN eltT : fifoEltK ty <- ^"elt";
-       Assert !$$(listIsEmpty eltT);
-       Write ^"elt" <- (Var _ (fifoEltK ty) (listDeq eltT));
-       Ret (listFirstElt eltT))%kami_action.
+  Definition fifoDeq: MethodT {| arg := Void; ret := dType |} :=
+    fun _ _ =>
+      (Read isFull <- ^"full";
+       Assert #isFull;
+       Read elt <- ^"elt";
+       Write ^"full" <- $$false;
+       Ret #elt)%kami_action.
 
-  Definition fifoFirstElt: forall ty (_: ty Void), ActionT ty dType :=
-    fun ty _ =>
-      (ReadN elt : fifoEltK ty <- ^"elt";
-       Assert !$$(listIsEmpty elt);
-       Ret (listFirstElt elt))%kami_action.
+  Definition fifoFirstElt: MethodT {| arg := Void; ret := dType |} :=
+    fun _ _ =>
+      (Read isFull <- ^"full";
+       Assert #isFull;
+       Read elt <- ^"elt";
+       Ret #elt)%kami_action.
+
+  Definition fifoIsFull: MethodT {| arg := Void; ret := Bool |} :=
+    fun _ _ =>
+      (Read isFull <- ^"full";
+       Ret #isFull)%kami_action.
+
+  Definition fifoClear: MethodT {| arg := Void; ret := Void |} :=
+    fun _ _ =>
+      (Write ^"full" <- $$false;
+       Retv)%kami_action.
 
   Definition fifo: Modules :=
     PrimMod
       {| pm_name := primFifoName;
          pm_regInits :=
-           [(^"elt" :: (RegInitCustom (existT ConstFullT (fifoEltK type)
-                                              (NativeConst nil nil))))%struct];
+           [^"elt" :: (RegInitDefault (SyntaxKind dType));
+              ^"full" :: (RegInitDefault (SyntaxKind dType))]%struct;
          pm_rules := nil;
          pm_methods :=
-           [(^"enq" :: (existT _ {| arg:= _; ret:= _ |} fifoEnq))%struct;
-              (^"deq" :: (existT _ {| arg:= _; ret:= _ |} fifoDeq))%struct;
-              (^"firstElt" :: (existT _ {| arg:= _; ret:= _ |} fifoFirstElt))%struct]
+           [^"enq" :: (existT _ _ fifoEnq);
+              ^"deq" :: (existT _ _ fifoDeq)]%struct
       |}.
 
-  Definition simpleFifo: Modules :=
+  Definition fifoF: Modules :=
     PrimMod
       {| pm_name := primFifoName;
          pm_regInits :=
-           [(^"elt" :: (RegInitCustom (existT ConstFullT (fifoEltK type)
-                                              (NativeConst nil nil))))%struct];
+           [^"elt" :: (RegInitDefault (SyntaxKind dType));
+              ^"full" :: (RegInitDefault (SyntaxKind dType))]%struct;
          pm_rules := nil;
          pm_methods :=
-           [(^"enq" :: (existT _ {| arg:= _; ret:= _ |} fifoEnq))%struct;
-              (^"deq" :: (existT _ {| arg:= _; ret:= _ |} fifoDeq))%struct]
+           [^"enq" :: (existT _ _ fifoEnq);
+              ^"deq" :: (existT _ _ fifoDeq);
+              ^"isFull" :: (existT _ _ fifoIsFull)]%struct
+      |}.
+
+  Definition fifoC: Modules :=
+    PrimMod
+      {| pm_name := primFifoName;
+         pm_regInits :=
+           [^"elt" :: (RegInitDefault (SyntaxKind dType));
+              ^"full" :: (RegInitDefault (SyntaxKind dType))]%struct;
+         pm_rules := nil;
+         pm_methods :=
+           [^"enq" :: (existT _ _ fifoEnq);
+              ^"deq" :: (existT _ _ fifoDeq);
+              ^"clear" :: (existT _ _ fifoClear)]%struct
       |}.
 
 End PrimFifo.
 
-Hint Unfold fifo simpleFifo : ModuleDefs.
-Hint Unfold listIsEmpty listIsFull listEnq listDeq listFirstElt
-     primFifoName fifoEltT fifoEltK fifoElt
-     fifoEnq fifoDeq fifoFirstElt: MethDefs.
+Hint Unfold fifo fifoF fifoC: ModuleDefs.
+Hint Unfold primFifoName
+     fifoEnq fifoDeq fifoFirstElt fifoIsFull fifoClear: MethDefs.
 
 Section Facts.
   Variables (fifoName: string)
-            (sz: nat)
             (dType: Kind).
 
   Lemma fifo_ModEquiv:
-    ModPhoasWf (fifo fifoName sz dType).
+    ModPhoasWf (fifo fifoName dType).
   Proof.
     kequiv.
   Qed.
   Hint Resolve fifo_ModEquiv.
 
-  Lemma simpleFifo_ModEquiv:
-    ModPhoasWf (simpleFifo fifoName sz dType).
+  Lemma fifoF_ModEquiv:
+    ModPhoasWf (fifoF fifoName dType).
   Proof.
     kequiv.
   Qed.
-  Hint Resolve simpleFifo_ModEquiv.
+  Hint Resolve fifoF_ModEquiv.
+
+  Lemma fifoC_ModEquiv:
+    ModPhoasWf (fifoC fifoName dType).
+  Proof.
+    kequiv.
+  Qed.
+  Hint Resolve fifoC_ModEquiv.
 
   Lemma fifo_ValidRegs:
-    ModRegsWf (fifo fifoName sz dType).
+    ModRegsWf (fifo fifoName dType).
   Proof.
     kvr.
   Qed.
   Hint Resolve fifo_ValidRegs.
 
-  Lemma simpleFifo_ValidRegs:
-    ModRegsWf (simpleFifo fifoName sz dType).
+  Lemma fifoF_ValidRegs:
+    ModRegsWf (fifoF fifoName dType).
   Proof.
     kvr.
   Qed.
-  Hint Resolve simpleFifo_ValidRegs.
+  Hint Resolve fifoF_ValidRegs.
+
+  Lemma fifoC_ValidRegs:
+    ModRegsWf (fifoC fifoName dType).
+  Proof.
+    kvr.
+  Qed.
+  Hint Resolve fifoC_ValidRegs.
 
 End Facts.
 
-Hint Resolve fifo_ModEquiv simpleFifo_ModEquiv.
-Hint Resolve fifo_ValidRegs simpleFifo_ValidRegs.
+Hint Resolve fifo_ModEquiv fifoF_ModEquiv fifoC_ModEquiv.
+Hint Resolve fifo_ValidRegs fifoF_ValidRegs fifoC_ValidRegs.
 
